aneris/aneris_lang/lifting.v
@@ -533,11 +533,11 @@ Section primitive_laws.
     iApply "HΦ"; done.
   Qed.
 
-  Lemma wp_start ip ports k E ζ e Φ :
+  Lemma wp_start ip k E ζ e Φ :
     ▷ is_node "system" ∗
     ▷ free_ip ip ∗
     ▷ Φ (mkVal "system" #()) ∗
-    ▷ (∀ tid, is_node ip -∗ free_ports ip ports -∗ WP (mkExpr ip e) @ k; (ip, tid); ⊤ {{ _, True }})
+    ▷ (∀ tid, is_node ip -∗ WP (mkExpr ip e) @ k; (ip, tid); ⊤ {{ _, True }})
     ⊢ WP mkExpr "system" (Start (LitString ip) e) @ k; ζ; E {{ Φ }}.
   Proof.
     iIntros "(>Hnode & >Hfip & HΦ & Hwp)".
@@ -557,8 +557,7 @@ Section primitive_laws.
     eapply aneris_events_state_interp_no_triggered in Htrig;
       [|done|done|done|done|done].
     inv_head_step.
-    iMod (aneris_state_interp_alloc_node _ _ ports with "[$]")
-      as "(%Hcoh & Hn & Hports & Hσ)".
+    iMod (aneris_state_interp_alloc_node with "[$]") as "(%Hcoh & Hn & Hσ)".
     iMod (steps_auth_update_S with "Hauth") as "Hauth".
     iModIntro.
     simplify_eq /=.
@@ -567,7 +566,7 @@ Section primitive_laws.
     rewrite Htrig; iFrame.
     iSplit; [ iPureIntro; apply user_model_evolution_id |].
     iSplitL "HΦ"; [by iApply wp_value|].
-    iSplitL; [ by iApply ("Hwp" with "[$] [$]")|done].
+    iSplitL; [ by iApply ("Hwp" with "[$]")|done].
   Qed. 
 
   Lemma wp_new_socket ip s E ζ :
