aneris/aneris_lang/no_model.v
@@ -9,13 +9,14 @@ Proof. intros ?. apply finite_smaller_card_nat. apply _. Qed.
 
 #[global] Notation anerisG Σ := (anerisG unit_model Σ).
 
-Theorem adequacy_hoare_no_model Σ `{anerisPreG Σ unit_model} IPs A lbls obs_send_sas obs_rec_sas e σ φ ip :
+Theorem adequacy_hoare_no_model Σ `{anerisPreG Σ unit_model} IPs ports A lbls obs_send_sas obs_rec_sas e σ φ ip :
   obs_send_sas ⊆ A →
   obs_rec_sas ⊆ A →
   (∀ `{anerisG Σ}, ⊢
           {{{ unallocated A ∗
               ([∗ set] a ∈ A, a ⤳[bool_decide (a ∈ obs_send_sas), bool_decide (a ∈ obs_rec_sas)] (∅, ∅)) ∗
               ([∗ set] ip ∈ IPs, free_ip ip) ∗
+              ([∗ map] ip↦p ∈ ports, free_ports ip p) ∗
               ([∗ set] lbl ∈ lbls, alloc_evs lbl []) ∗
               ([∗ set] sa ∈ obs_send_sas, sendon_evs sa []) ∗
               ([∗ set] sa ∈ obs_rec_sas, receiveon_evs sa []) ∗
@@ -31,44 +32,50 @@ Theorem adequacy_hoare_no_model Σ `{anerisPreG Σ unit_model} IPs A lbls obs_se
   aneris_adequate e ip σ φ.
 Proof.
   intros ?? Hspec ?????.
-  eapply (adequacy_hoare Σ _ IPs A lbls obs_send_sas obs_rec_sas);
+  eapply (adequacy_hoare Σ _ IPs ports A lbls obs_send_sas obs_rec_sas);
     [set_solver|set_solver|..|done|set_solver|set_solver|set_solver|done].
   { apply unit_model_rel_finitary. }
-  iIntros (? Φ) "!# (?&?&?&?&?&?&?&?&?) HΦ".
+  iIntros (? Φ) "!# (?&?&?&?&?&?&?&?&?&?) HΦ".
   iApply (Hspec with "[-HΦ]"); [|done].
   iFrame.
 Qed.
 
-Lemma adequacy_hoare_no_model_simpl_helper Σ `{anerisPreG Σ unit_model} IPs A e φ ip: 
-(∀ `{anerisG Σ}, ⊢
-{{{ unallocated A ∗ ([∗ set] a ∈ A, a ⤳ (∅, ∅)) ∗ ([∗ set] ip ∈ IPs, free_ip ip)}}}
-    e @[ip]
-{{{ v, RET v; ⌜φ v⌝ }}}) →
-∃ lbls obs_send_sas obs_rec_sas, 
-obs_send_sas ⊆ A ∧ 
-obs_rec_sas ⊆ A ∧
-(∀ `{anerisG Σ}, ⊢
-          {{{ unallocated A ∗
-              ([∗ set] a ∈ A, a ⤳[bool_decide (a ∈ obs_send_sas), bool_decide (a ∈ obs_rec_sas)] (∅, ∅)) ∗
-              ([∗ set] ip ∈ IPs, free_ip ip) ∗
-              ([∗ set] lbl ∈ lbls, alloc_evs lbl []) ∗
-              ([∗ set] sa ∈ obs_send_sas, sendon_evs sa []) ∗
-              ([∗ set] sa ∈ obs_rec_sas, receiveon_evs sa []) ∗
-              observed_send obs_send_sas ∗
-              observed_receive obs_rec_sas }}}
-          e @[ip]
+Lemma adequacy_hoare_no_model_simpl_helper Σ `{anerisPreG Σ unit_model} IPs ports A e φ ip: 
+  (∀ `{anerisG Σ}, ⊢
+                   {{{ unallocated A ∗ ([∗ set] a ∈ A, a ⤳ (∅, ∅)) ∗
+                       ([∗ map] ip↦p ∈ ports, free_ports ip p) ∗
+                       ([∗ set] ip ∈ IPs, free_ip ip) }}}
+                     e @[ip]
+                     {{{ v, RET v; ⌜φ v⌝ }}}) →
+  ∃ lbls obs_send_sas obs_rec_sas,
+    obs_send_sas ⊆ A ∧
+    obs_rec_sas ⊆ A ∧
+    (∀ `{anerisG Σ}, ⊢
+      {{{ unallocated A ∗
+          ([∗ set] a ∈ A, a ⤳[bool_decide (a ∈ obs_send_sas),
+                              bool_decide (a ∈ obs_rec_sas)] (∅, ∅)) ∗
+          ([∗ set] ip ∈ IPs, free_ip ip) ∗
+          ([∗ map] ip↦p ∈ ports, free_ports ip p) ∗
+          ([∗ set] lbl ∈ lbls, alloc_evs lbl []) ∗
+          ([∗ set] sa ∈ obs_send_sas, sendon_evs sa []) ∗
+          ([∗ set] sa ∈ obs_rec_sas, receiveon_evs sa []) ∗
+          observed_send obs_send_sas ∗
+          observed_receive obs_rec_sas }}}
+        e @[ip]
       {{{ v, RET v; ⌜φ v⌝ }}}).
 Proof.
   intros Ht. exists ∅, ∅, ∅. 
   do 2 (split; try done).
   iIntros (? ?) "!# HPre HPost". 
   iApply (Ht with "[HPre] [HPost]"); try done.
-  iDestruct "HPre" as "[? [? [? ?]]]". iFrame.
+  iDestruct "HPre" as "(?&?&?&?&?&?)". iFrame.
 Qed.     
 
-Theorem adequacy_hoare_no_model_simpl Σ `{anerisPreG Σ unit_model} IPs A e σ φ ip :
+Theorem adequacy_hoare_no_model_simpl Σ `{anerisPreG Σ unit_model} IPs ports A e σ φ ip :
   (∀ `{anerisG Σ}, ⊢
-      {{{ unallocated A ∗ ([∗ set] a ∈ A, a ⤳ (∅, ∅)) ∗ ([∗ set] ip ∈ IPs, free_ip ip)}}}
+      {{{ unallocated A ∗ ([∗ set] a ∈ A, a ⤳ (∅, ∅)) ∗
+          ([∗ map] ip↦p ∈ ports, free_ports ip p) ∗
+          ([∗ set] ip ∈ IPs, free_ip ip) }}}
           e @[ip]
       {{{ v, RET v; ⌜φ v⌝ }}}) →
   ip ∉ IPs →
@@ -81,5 +88,5 @@ Proof.
   intros Ht ?????. 
   apply adequacy_hoare_no_model_simpl_helper in Ht; try done.
   destruct Ht as [lbls[obs_send_sas[obs_rec_sas[HSend [HRec Ht]]]]].
-  by eapply (adequacy_hoare_no_model Σ IPs A lbls obs_send_sas obs_rec_sas).
+  by eapply (adequacy_hoare_no_model Σ IPs ports A lbls obs_send_sas obs_rec_sas).
 Qed.
