aneris/aneris_lang/program_logic/aneris_adequacy.v
@@ -9,7 +9,7 @@ Definition aneris_adequate (e :expr) (ip : ip_address) (σ : state)
   adequate NotStuck (mkExpr ip e) σ (λ v _, ∃ w, v = mkVal ip w ∧ φ w).
 
 Theorem adequacy_groups Σ Mdl `{anerisPreG Σ Mdl} `{EqDecision (aneris_to_trace_model Mdl)}
-        IPs A lbls obs_send_sas obs_rec_sas e ip σ φ :
+        IPs ports A lbls obs_send_sas obs_rec_sas e ip σ φ :
   all_disjoint A →
   set_Forall (λ sag, sag ≠ ∅) A →
   obs_send_sas ⊆ A → obs_rec_sas ⊆ A →
@@ -19,6 +19,7 @@ Theorem adequacy_groups Σ Mdl `{anerisPreG Σ Mdl} `{EqDecision (aneris_to_trac
      ([∗ set] b ∈ A, b ⤳*[bool_decide (b ∈ obs_send_sas), bool_decide (b ∈ obs_rec_sas)] (∅, ∅)) -∗
      frag_st Mdl.(model_state_initial) -∗
      ([∗ set] i ∈ IPs, free_ip i) -∗
+     ([∗ map] ip↦p ∈ ports, free_ports ip p) -∗
      ([∗ set] lbl ∈ lbls, alloc_evs lbl []) -∗
      ([∗ set] sa ∈ obs_send_sas, sendon_evs_groups sa []) -∗
      ([∗ set] sa ∈ obs_rec_sas, receiveon_evs_groups sa []) -∗
@@ -34,25 +35,26 @@ Theorem adequacy_groups Σ Mdl `{anerisPreG Σ Mdl} `{EqDecision (aneris_to_trac
 Proof.
   intros Hdisj Hne Hsendle Hrecvle.
   intros HMdlfin Hwp Hip Hfixdom Hste Hsce Hmse.
-  eapply (adequacy_groups _ A _ obs_send_sas obs_rec_sas);
+  eapply (adequacy_groups _ _ A _ obs_send_sas obs_rec_sas);
     [done|done|done|done|done| |done|done|done|done|done].
   intros dg.
   iMod (Hwp dg) as "Hwp".
-  iModIntro. iIntros "?????????? /=".
+  iModIntro. iIntros "??????????? /=".
   rewrite !aneris_wp_unfold /aneris_wp_def.
-  iSpecialize ("Hwp" with "[$] [$] [$] [$] [$] [$] [$] [$] [$] [$]").
+  iSpecialize ("Hwp" with "[$] [$] [$] [$] [$] [$] [$] [$] [$] [$] [$]").
   iApply (wp_wand with "Hwp").
   eauto.
 Qed.
 
 Theorem adequacy1 Σ Mdl `{anerisPreG Σ Mdl} `{EqDecision (aneris_to_trace_model Mdl)}
-        IPs A lbls obs_send_sas obs_rec_sas e ip σ φ :
+        IPs ports A lbls obs_send_sas obs_rec_sas e ip σ φ :
   aneris_model_rel_finitary Mdl →
   (∀ `{anerisG Mdl Σ}, ⊢ |={⊤}=>
      unallocated A -∗
      ([∗ set] a ∈ A, a ⤳1[bool_decide (a ∈ obs_send_sas), bool_decide (a ∈ obs_rec_sas)] (∅, ∅)) -∗
      frag_st Mdl.(model_state_initial) -∗
      ([∗ set] i ∈ IPs, free_ip i) -∗
+     ([∗ map] ip↦p ∈ ports, free_ports ip p) -∗
      ([∗ set] lbl ∈ lbls, alloc_evs lbl []) -∗
      ([∗ set] sa ∈ obs_send_sas, sendon_evs sa []) -∗
      ([∗ set] sa ∈ obs_rec_sas, receiveon_evs sa []) -∗
@@ -71,21 +73,22 @@ Proof.
   eapply adequacy1; [done| |apply Hsendle|done|done|done|done|done|done].
   intros dg.
   iMod (Hwp dg) as "Hwp".
-  iModIntro. iIntros "?????????? /=".
+  iModIntro. iIntros "??????????? /=".
   rewrite !aneris_wp_unfold /aneris_wp_def.
-  iSpecialize ("Hwp" with "[$] [$] [$] [$] [$] [$] [$] [$] [$] [$]").
+  iSpecialize ("Hwp" with "[$] [$] [$] [$] [$] [$] [$] [$] [$] [$] [$]").
   iApply (wp_wand with "Hwp").
   eauto.
 Qed.
 
 Theorem adequacy Σ Mdl `{anerisPreG Σ Mdl} `{EqDecision (aneris_to_trace_model Mdl)}
-        IPs A lbls obs_send_sas obs_rec_sas e ip σ φ :
+        IPs ports A lbls obs_send_sas obs_rec_sas e ip σ φ :
   aneris_model_rel_finitary Mdl →
   (∀ `{anerisG Mdl Σ}, ⊢ |={⊤}=>
      unallocated A -∗
      ([∗ set] a ∈ A, a ⤳[bool_decide (a ∈ obs_send_sas), bool_decide (a ∈ obs_rec_sas)] (∅, ∅)) -∗
      frag_st Mdl.(model_state_initial) -∗
      ([∗ set] i ∈ IPs, free_ip i) -∗
+     ([∗ map] ip↦p ∈ ports, free_ports ip p) -∗
      ([∗ set] lbl ∈ lbls, alloc_evs lbl []) -∗
      ([∗ set] sa ∈ obs_send_sas, sendon_evs sa []) -∗
      ([∗ set] sa ∈ obs_rec_sas, receiveon_evs sa []) -∗
@@ -104,15 +107,15 @@ Proof.
   eapply adequacy; [done| |apply Hsendle|done|done|done|done|done|done].
   intros dg.
   iMod (Hwp dg) as "Hwp".
-  iModIntro. iIntros "?????????? /=".
+  iModIntro. iIntros "??????????? /=".
   rewrite !aneris_wp_unfold /aneris_wp_def.
-  iSpecialize ("Hwp" with "[$] [$] [$] [$] [$] [$] [$] [$] [$] [$]").
+  iSpecialize ("Hwp" with "[$] [$] [$] [$] [$] [$] [$] [$] [$] [$] [$]").
   iApply (wp_wand with "Hwp").
   eauto.
 Qed.
 
 Theorem adequacy_hoare_groups Σ Mdl `{anerisPreG Σ Mdl} `{EqDecision (aneris_to_trace_model Mdl)}
-        IPs A lbls obs_send_sas obs_rec_sas e σ φ ip :
+        IPs ports A lbls obs_send_sas obs_rec_sas e σ φ ip :
   all_disjoint A →
   set_Forall (λ sag, sag ≠ ∅) A →
   obs_send_sas ⊆ A → obs_rec_sas ⊆ A →
@@ -122,6 +125,7 @@ Theorem adequacy_hoare_groups Σ Mdl `{anerisPreG Σ Mdl} `{EqDecision (aneris_t
               ([∗ set] a ∈ A, a ⤳*[bool_decide (a ∈ obs_send_sas), bool_decide (a ∈ obs_rec_sas)] (∅, ∅)) ∗
               frag_st Mdl.(model_state_initial) ∗
               ([∗ set] ip ∈ IPs, free_ip ip) ∗
+              ([∗ map] ip↦p ∈ ports, free_ports ip p) ∗
               ([∗ set] lbl ∈ lbls, alloc_evs lbl []) ∗
               ([∗ set] sa ∈ obs_send_sas, sendon_evs_groups sa []) ∗
               ([∗ set] sa ∈ obs_rec_sas, receiveon_evs_groups sa []) ∗
@@ -138,15 +142,15 @@ Theorem adequacy_hoare_groups Σ Mdl `{anerisPreG Σ Mdl} `{EqDecision (aneris_t
 Proof.
   intros Hdisj Hne Hsendle Hrecvle.
   intros ? Hwp ?????.
-  eapply (adequacy_groups _ _ _ A _ obs_send_sas obs_rec_sas); eauto.
+  eapply (adequacy_groups _ _ _ ports A _ obs_send_sas obs_rec_sas); eauto.
   intros ?. iModIntro.
   iDestruct Hwp as "#Hwp".
-  iIntros "?????????".
+  iIntros "??????????".
   iApply ("Hwp" with "[$]"); auto.
 Qed.
 
 Theorem adequacy1_hoare Σ Mdl `{anerisPreG Σ Mdl} `{EqDecision (aneris_to_trace_model Mdl)}
-        IPs A lbls obs_send_sas obs_rec_sas e σ φ ip :
+        IPs ports A lbls obs_send_sas obs_rec_sas e σ φ ip :
   obs_send_sas ⊆ A → obs_rec_sas ⊆ A →
   aneris_model_rel_finitary Mdl →
   (∀ `{anerisG Mdl Σ}, ⊢
@@ -154,6 +158,7 @@ Theorem adequacy1_hoare Σ Mdl `{anerisPreG Σ Mdl} `{EqDecision (aneris_to_trac
               ([∗ set] a ∈ A, a ⤳1[bool_decide (a ∈ obs_send_sas), bool_decide (a ∈ obs_rec_sas)] (∅, ∅)) ∗
               frag_st Mdl.(model_state_initial) ∗
               ([∗ set] ip ∈ IPs, free_ip ip) ∗
+              ([∗ map] ip↦p ∈ ports, free_ports ip p) ∗
               ([∗ set] lbl ∈ lbls, alloc_evs lbl []) ∗
               ([∗ set] sa ∈ obs_send_sas, sendon_evs sa []) ∗
               ([∗ set] sa ∈ obs_rec_sas, receiveon_evs sa []) ∗
@@ -169,15 +174,15 @@ Theorem adequacy1_hoare Σ Mdl `{anerisPreG Σ Mdl} `{EqDecision (aneris_to_trac
   aneris_adequate e ip σ φ.
 Proof.
   intros ??? Hwp ?????.
-  eapply (adequacy1 _ _ _ _ _ obs_send_sas obs_rec_sas); eauto.
+  eapply (adequacy1 _ _ _ _ _ _ obs_send_sas obs_rec_sas); eauto.
   intros ?. iModIntro.
   iDestruct Hwp as "#Hwp".
-  iIntros "?????????".
+  iIntros "??????????".
   iApply ("Hwp" with "[$]"); auto.
 Qed.
 
 Theorem adequacy_hoare Σ Mdl `{anerisPreG Σ Mdl} `{EqDecision (aneris_to_trace_model Mdl)}
-        IPs A lbls obs_send_sas obs_rec_sas e σ φ ip :
+        IPs ports A lbls obs_send_sas obs_rec_sas e σ φ ip :
   obs_send_sas ⊆ A → obs_rec_sas ⊆ A →
   aneris_model_rel_finitary Mdl →
   (∀ `{anerisG Mdl Σ}, ⊢
@@ -185,6 +190,7 @@ Theorem adequacy_hoare Σ Mdl `{anerisPreG Σ Mdl} `{EqDecision (aneris_to_trace
               ([∗ set] a ∈ A, a ⤳[bool_decide (a ∈ obs_send_sas), bool_decide (a ∈ obs_rec_sas)] (∅, ∅)) ∗
               frag_st Mdl.(model_state_initial) ∗
               ([∗ set] ip ∈ IPs, free_ip ip) ∗
+              ([∗ map] ip↦p ∈ ports, free_ports ip p) ∗
               ([∗ set] lbl ∈ lbls, alloc_evs lbl []) ∗
               ([∗ set] sa ∈ obs_send_sas, sendon_evs sa []) ∗
               ([∗ set] sa ∈ obs_rec_sas, receiveon_evs sa []) ∗
@@ -200,9 +206,9 @@ Theorem adequacy_hoare Σ Mdl `{anerisPreG Σ Mdl} `{EqDecision (aneris_to_trace
   aneris_adequate e ip σ φ.
 Proof.
   intros ??? Hwp ?????.
-  eapply (adequacy _ _ _ _ _ obs_send_sas obs_rec_sas); eauto.
+  eapply (adequacy _ _ _ _ _ _ obs_send_sas obs_rec_sas); eauto.
   intros ?. iModIntro.
   iDestruct Hwp as "#Hwp".
-  iIntros "?????????".
+  iIntros "??????????".
   iApply ("Hwp" with "[$]"); auto.
 Qed.
