aneris/aneris_lang/state_interp/state_interp_config_wp.v
@@ -8,6 +8,7 @@ From aneris.aneris_lang.state_interp Require Import
      state_interp_local_coh
      state_interp_gnames_coh
      state_interp_free_ips_coh
+     state_interp_free_ports_coh
      state_interp_network_sockets_coh
      state_interp_socket_interp_coh
      state_interp_messages_resource_coh
@@ -66,7 +67,9 @@ Section state_interpretation.
                 eauto using messages_history_coh_deliver_message|].
       iSplitL "Hlcoh";
         [by iApply (local_state_coh_deliver_message with "Hlcoh")|].
-      iApply free_ips_coh_ms. by iApply free_ips_coh_deliver_message.
+      iSplitL "Hfreeips";
+        [by iApply free_ips_coh_ms; iApply free_ips_coh_update_sockets|].
+      by iApply free_ports_coh_update; iApply free_ports_coh_update_socket.
     - iFrame.
       iSplit.
       { iPureIntro.
