aneris/aneris_lang/state_interp/state_interp_free_ports_coh.v
@@ -1,0 +1,157 @@
+From stdpp Require Import fin_maps gmap.
+From iris.bi.lib Require Import fractional.
+From iris.proofmode Require Import tactics.
+From iris.base_logic.lib Require Import saved_prop gen_heap.
+From aneris.lib Require Import gen_heap_light.
+From aneris.aneris_lang Require Import
+     aneris_lang network resources.
+From aneris.aneris_lang.state_interp Require Import
+     state_interp_def.
+
+From RecordUpdate Require Import RecordSet.
+Set Default Proof Using "Type".
+
+Import uPred.
+Import RecordSetNotations.
+
+Section state_interpretation.
+  Context `{!anerisG Mdl Σ}.
+
+  Lemma free_ports_coh_init free_ports σ :
+    (map_Forall (λ ip ports,
+                     (∀ Sn, (state_sockets σ) !! ip = Some Sn →
+                            set_Forall (λ p, port_not_in_use p Sn) ports))
+                free_ports) →
+    free_ports_auth free_ports -∗
+    free_ports_coh σ.
+  Proof. iIntros (?) "?". by iExists _; iFrame. Qed.
+
+  Lemma free_ports_coh_free_ports_valid σ a Sn :
+    state_sockets σ !! ip_of_address a = Some Sn →
+    free_ports_coh σ -∗
+    free_ports (ip_of_address a) {[port_of_address a]} -∗
+    ⌜port_not_in_use (port_of_address a) Sn⌝.
+  Proof.
+    iIntros (Hskts). iDestruct 1 as (ports Hports) "HpCtx". iIntros "Hp".
+    iDestruct (free_ports_included with "HpCtx Hp") as (?) "[%Hlookup %]".
+    iPureIntro.
+    eapply Hports; [done|done|set_solver].
+  Qed.
+
+  Lemma free_ports_coh_alloc_node ip σ :
+    state_sockets σ !! ip = None →
+    free_ports_coh σ -∗
+    free_ports_coh (σ <| state_sockets := <[ip := ∅]> (state_sockets σ) |>).
+  Proof.
+    intros Hip.
+    iDestruct 1 as (ps Hps) "HpsCtx".
+    iExists _. iFrame. iPureIntro.
+    intros ip' ps' HSome' Sn' HPs'.
+    destruct (decide (ip = ip')); simplify_map_eq.
+    - intros ???????. set_solver.
+    - by eapply Hps.
+  Qed.
+
+  Lemma free_ports_coh_alloc_socket ip σ Sn sh s r :
+    state_sockets σ !! ip = Some Sn →
+    Sn !! sh = None →
+    saddress s = None →
+    free_ports_coh σ -∗
+    free_ports_coh
+      (σ <| state_sockets :=
+         <[ip := <[sh := (s,r)]>Sn]>
+           (state_sockets σ) |>).
+  Proof.
+    intros Hip.
+    iDestruct 1 as (ps Hps) "HpsCtx".
+    iExists _. iFrame. iPureIntro.
+    intros ip' ps' HSome' Sn' HPs'.
+    destruct (decide (ip = ip')); simplify_map_eq.
+    - intros p Hin sh' skt' a' r' Hsh' Haddr.
+      destruct (decide (sh = sh')) as [->|Hneq].
+      + rewrite lookup_insert in Hsh'. simplify_eq.
+      + rewrite lookup_insert_ne in Hsh'; [|done]. by eapply Hps.
+    - by eapply Hps.
+  Qed.
+
+  Lemma free_ports_coh_update_socket sh ip skt1 skt2 Sn r1 r2 σ1 :
+    state_sockets σ1 !! ip = Some Sn →
+    Sn !! sh = Some (skt1, r1) →
+    saddress skt1 = saddress skt2 →
+    free_ports_coh σ1 -∗
+    free_ports_coh
+      (σ1 <| state_sockets :=
+         <[ip := <[sh:=(skt2, r2)]> Sn]>
+                     (state_sockets σ1) |>).
+  Proof.
+    destruct skt1, skt2.
+    intros Hskt HSn Hsh.
+    iDestruct 1 as (ps Hps) "HpsCtx".
+    iExists _. iFrame. iPureIntro.
+    intros ip' ps' HSome' Sn' HPs'.
+    destruct (decide (ip = ip')); simplify_map_eq.
+    - intros p Hin.
+      intros sh' skt' a' r' Hsh' Haddr.
+      destruct (decide (sh = sh')) as [->|Hneq].
+      + rewrite lookup_insert in Hsh'. simplify_eq. simpl in Haddr.
+        simplify_eq. by eapply Hps.
+      + rewrite lookup_insert_ne in Hsh'; [|done]. by eapply Hps.
+    - by eapply Hps.
+  Qed.
+
+  (* Special case of [free_ports_coh_update_socket]
+     that matches some goals better syntactically *)
+  Lemma free_ports_coh_update_sblock sh ip skt b Sn r1 r2 σ1 :
+    state_sockets σ1 !! ip = Some Sn →
+    Sn !! sh = Some (skt, r1) →
+    free_ports_coh σ1 -∗
+    free_ports_coh
+      (σ1 <| state_sockets :=
+         <[ip := <[sh:=(skt<| sblock := b|>, r2)]> Sn]>
+                     (state_sockets σ1) |>).
+  Proof. iIntros (??) "?". by iApply free_ports_coh_update_socket. Qed.
+
+  Lemma free_ports_coh_bind_socket σ1 a r sh skt Sn :
+    state_sockets σ1 !! ip_of_address a = Some Sn →
+    free_ports_coh σ1 -∗
+    free_ports (ip_of_address a) {[port_of_address a]} ==∗
+    free_ports_coh
+      (σ1 <| state_sockets :=
+         <[ip_of_address a :=
+             <[sh:=(skt<| saddress := Some a |>, r)]> Sn]>
+                 (state_sockets σ1) |>).
+  Proof.
+    intros HSome.
+    iDestruct 1 as (Ps HPs) "HpCtx".
+    iIntros "Hp".
+    iMod (free_ports_dealloc with "HpCtx Hp")
+      as (ps [Hps' Hin%elem_of_subseteq_singleton]) "HpCtx".
+    iModIntro. iExists _; iFrame. iPureIntro.
+    intros ip' ps' HSome' Sn' HPs'.
+    destruct (decide (ip_of_address a = ip')); simplify_map_eq.
+    - intros p [Hin' Hnin%not_elem_of_singleton]%elem_of_difference.
+      intros sh' skt' a' r' Hsh' Haddr. simplify_eq.
+      destruct (decide (sh = sh')) as [->|Hneq].
+      + rewrite lookup_insert in Hsh'. simplify_eq. simpl in Haddr.
+        by simplify_eq.
+      + rewrite lookup_insert_ne in Hsh'; [|done]. by eapply HPs.
+    - by eapply HPs.
+  Qed.
+
+  Lemma free_ports_coh_update hps1 hps2 skts ms1 ms2 :
+    free_ports_coh {|
+      state_heaps := hps1;
+      state_sockets := skts;
+      state_ms := ms1;
+      |} -∗
+    free_ports_coh {|
+      state_heaps := hps2;
+      state_sockets := skts;
+      state_ms := ms2;
+    |}.
+  Proof.
+    iDestruct 1 as (ps Hps) "HpsCtx".
+    iExists _. by iFrame.
+  Qed.
+
+End state_interpretation.
